heap/tree_pop.v
@@ -16,6 +16,7 @@ Require Import cprogs.heap.definitions.
 Require Import cprogs.heap.tree_list.
 Require Import cprogs.heap.tree_down.
 Require Import cprogs.heap.math_prop.
+Require Import cprogs.heap.tree_push.
 
 Fixpoint tree_to_partial_tree_pop_fix (tl: partial_tree) (t: tree) (d: Z): partial_tree :=
   match t with
@@ -33,19 +34,27 @@ Definition tree_to_partial_tree_pop(t: tree) (d: Z): partial_tree :=
 Definition get_last_val(l: partial_tree): Z :=
   match l with
     | nil => 0
-    | (flg, v, tr)::lt => v
+    | (flg, v, tr) :: lt => v
   end.
 
 Definition tree_cut_last(ls rs: tree) (d: Z): tree :=
   if (full_tree_b (d - 2) rs) then
     (Node (get_last_val (tree_to_partial_tree_pop ls (d-1)))
         (tree_compose (skipn 1%nat (tree_to_partial_tree_pop ls (d-1))) Leaf) rs)
-  else (Node (get_last_val ( tree_to_partial_tree_pop rs (d-1)))
+  else (Node (get_last_val (tree_to_partial_tree_pop rs (d-1)))
         ls (tree_compose (skipn 1%nat (tree_to_partial_tree_pop rs (d-1))) Leaf)).
 
 Definition tree_pop: tree -> tree -> Prop :=
-  fun t t' => (tree_size t <= 1  /\ t' = Leaf) \/ 
-    (exists v ls rs ts d, t = (Node v ls rs) /\ complete_tree_pop d t /\ heap_tree_down (nil,(tree_cut_last ls rs d)) ts /\ t' = (tree_compose (fst ts) (snd ts))).
+  fun t t' => (tree_size t <= 1  /\ t' = Leaf) \/
+    (tree_size t >= 2 /\ exists v ls rs ts d, t = (Node v ls rs) /\ complete_tree_pop d t /\ heap_tree_down (nil,(tree_cut_last ls rs d)) ts /\ t' = (tree_compose (fst ts) (snd ts))).
+
+Lemma tree_not_emp: forall (t: tree),
+  tree_size t >= 1 -> exists v ls rs, t = Node v ls rs.
+Proof.
+  intros.
+  induction t; simpl in *; try lia.
+  exists v, t1, t2; auto.
+Qed.
 
 Lemma complete_tree_pop_not_fullb: forall d t,
   complete_tree_pop d t -> full_tree_b (d - 1) t = false.
@@ -315,6 +324,193 @@ Proof.
   + unfold not; intros; discriminate. 
 Qed.
 
+Lemma MaxHeap_tree_partial_tree_skip: forall (lt: partial_tree),
+  MaxHeap_partial_tree lt -> MaxHeap_partial_tree (skipn 1 lt).
+Proof.
+  intros.
+  induction lt.
+  + simpl; tauto.
+  + destruct a as [[flg val] tr].
+    inversion H.
+    simpl.
+    apply (MaxHeap_partial_tree_v_impl _ val).
+    tauto.
+Qed.
+
+Lemma tree_to_partial_tree_pop_get: forall (t tr: tree) (lt: partial_tree) (flg: bool) (v d: Z), 
+  tree_to_partial_tree_pop_fix (lt ++ [(flg,v,tr)]) t d = (tree_to_partial_tree_pop_fix lt t d) ++ [(flg,v,tr)].
+Proof.
+  intros.
+  revert v tr flg d lt.
+  induction t; intros.
+  + unfold tree_to_partial_tree_pop_fix; tauto.
+  + simpl.
+    destruct (full_tree_b (d - 2) t2).
+    - replace ((false, v, t2) :: (lt ++ [(flg, v0, tr)])) with ([(false, v, t2)] ++ (lt ++ [(flg, v0, tr)])) by reflexivity.
+      replace ((false, v, t2) :: lt) with ([(false, v, t2)] ++ lt) by reflexivity.
+      rewrite app_assoc.
+      apply IHt1.
+    - replace ((true, v, t1) :: (lt ++ [(flg, v0, tr)])) with ([(true, v, t1)] ++ (lt ++ [(flg, v0, tr)])) by reflexivity.
+      replace ((true, v, t1) :: lt) with ([(true, v, t1)] ++ lt) by reflexivity.
+      rewrite app_assoc.
+      apply IHt2.
+Qed.
+
+Lemma MaxHeap_tree_partial_hold: forall (t: tree) (d: Z) (lt: partial_tree),
+  complete_tree_pop d t -> MaxHeap t -> (t = Leaf \/ MaxHeap_partial_tree_v lt (get_tree_val t)) -> MaxHeap_partial_tree lt -> 
+  MaxHeap_partial_tree (tree_to_partial_tree_pop_fix lt t d).
+Proof.
+  intros.
+  revert lt d H H2 H1.
+  induction H0; intros; subst.
+  + simpl; tauto.
+  + simpl; inversion H2; subst.
+    - apply full_tree_equiv1 in H8.
+      rewrite H8.
+      destruct H4; [discriminate|unfold get_tree_val in H].
+      apply IHMaxHeap1; [tauto| | ].
+      * unfold MaxHeap_partial_tree; tauto.
+      * destruct H0; [left; tauto|right].
+        eapply MaxHeap_partial_tree_v_app; try reflexivity; try tauto.
+    - pose proof complete_tree_pop_not_fullb _ _ H8.
+      replace (d-1-1) with (d-2) in H by lia.
+      rewrite H.
+      destruct H4; [discriminate|unfold get_tree_val in H4].
+      apply IHMaxHeap2; [tauto| | ].
+      * unfold MaxHeap_partial_tree; tauto.
+      * destruct H1; [left; tauto|right].
+        eapply MaxHeap_partial_tree_v_app; try reflexivity; try tauto.
+Qed.
+
+Lemma tree_to_partial_tree_len: forall (t: tree) (d: Z),
+  t <> Leaf -> 1 <= Zlength (tree_to_partial_tree_pop t d).
+Proof.
+  intros.
+  revert d.
+  induction t; [tauto|].
+  intros.
+  unfold tree_to_partial_tree_pop; simpl.
+  destruct (full_tree_b (d-2) t2); simpl.
+  + replace ((false, v, t2) :: nil) with (nil ++ [(false, v, t2)]); [|rewrite app_nil_l; tauto].
+    rewrite tree_to_partial_tree_pop_get.
+    rewrite Zlength_app.
+    replace (Zlength [(false, v, t2)]) with 1 by tauto.
+    pose proof initial_world.zlength_nonneg _ (tree_to_partial_tree_pop_fix [] t1 (d - 1)).
+    lia.
+  + replace ((true, v, t1) :: nil) with (nil ++ [(true, v, t1)]); [|rewrite app_nil_l; tauto].
+    rewrite tree_to_partial_tree_pop_get.
+    rewrite Zlength_app.
+    replace (Zlength [(true, v, t1)]) with 1 by tauto.
+    pose proof initial_world.zlength_nonneg _ (tree_to_partial_tree_pop_fix [] t2 (d - 1)).
+    lia.
+Qed.
+
+Lemma full_tree_gt_0: forall (t: tree) (d: Z),
+  full_tree d t -> d >= 0.
+Proof.
+  intros.
+  induction H.
+  + lia.
+  + lia.
+Qed.
+
+Lemma tree_compose_size_pop: forall (t: tree) (d: Z),
+  complete_tree_pop d t -> t <> Leaf -> tree_size
+  (tree_compose (skipn 1 (tree_to_partial_tree_pop t d)) Leaf) + 1 = tree_size t.
+Proof.
+  intros.
+  revert d H.
+  induction t; intros; [tauto|].
+  unfold tree_to_partial_tree_pop.
+  inversion H; subst.
+  + apply full_tree_equiv1 in H5.
+    unfold tree_to_partial_tree_pop_fix; fold tree_to_partial_tree_pop_fix.
+    rewrite H5.
+    destruct t1.
+    - inversion H3.
+      replace (d-2) with (-1) in H5 by lia.
+      apply full_tree_equiv1 in H5.
+      pose proof full_tree_gt_0 _ _ H5.
+      lia. 
+    - replace ((false, v, t2) :: nil) with (nil ++ [(false, v, t2)]); [|rewrite app_nil_l; tauto].
+      rewrite tree_to_partial_tree_pop_get.
+      replace 1%nat with (Z.to_nat 1) by lia.
+      pose proof tree_to_partial_tree_len (Node v0 t1_1 t1_2) (d-1).
+      unfold tree_to_partial_tree_pop in H1.
+      rewrite Zskipn_app1; [|apply H1; discriminate].
+      rewrite tree_compose_append.
+      unfold tree_size; fold tree_size.
+      unfold tree_to_partial_tree_pop in IHt1.
+      replace (Z.to_nat 1) with 1%nat by lia.
+      specialize (IHt1 ltac:(discriminate) (d-1) H3).
+      replace (tree_size (tree_compose (skipn 1 (tree_to_partial_tree_pop_fix [] (Node v0 t1_1 t1_2) (d - 1))) Leaf)) with (tree_size (Node v0 t1_1 t1_2) - 1) by lia.
+      simpl; lia.
+  + pose proof complete_tree_pop_not_fullb _ _ H5.
+    unfold tree_to_partial_tree_pop_fix; fold tree_to_partial_tree_pop_fix.
+    replace (d-1-1) with (d-2) in H1 by lia.
+    rewrite H1.
+    destruct t2.
+    - simpl.
+      inversion H3; [simpl; tauto|].
+      inversion H5.
+      replace (d-1-1) with (-1) in H2 by lia.
+      pose proof full_tree_gt_0 _ _ H2; lia.
+    - replace ((true, v, t1) :: nil) with (nil ++ [(true, v, t1)]); [|  rewrite app_nil_l; tauto].
+      rewrite tree_to_partial_tree_pop_get.
+      replace 1%nat with (Z.to_nat 1) by lia.
+      pose proof tree_to_partial_tree_len (Node v0 t2_1 t2_2) (d-1).
+      unfold tree_to_partial_tree_pop in H2.
+      rewrite Zskipn_app1; [|apply H2; discriminate].
+      rewrite tree_compose_append.
+      unfold tree_size; fold tree_size.
+      unfold tree_to_partial_tree_pop in IHt2.
+      replace (Z.to_nat 1) with 1%nat by lia.
+      specialize (IHt2 ltac:(discriminate) (d-1) H5).
+      replace (tree_size (tree_compose (skipn 1 (tree_to_partial_tree_pop_fix [] (Node v0 t2_1 t2_2) (d - 1))) Leaf)) with (tree_size (Node v0 t2_1 t2_2) - 1) by lia.
+      simpl; lia.
+Qed.
+
+Lemma tree_cut_last_size: forall (ls rs: tree) (v d: Z),
+  tree_size (Node v ls rs) >= 2 -> complete_tree_pop d (Node v ls rs) -> tree_size (tree_cut_last ls rs d) = tree_size ls + tree_size rs.
+Proof.
+  intros.
+  unfold tree_cut_last.
+  inversion H0; subst. 
+  + apply full_tree_equiv1 in H5; rewrite H5.
+    unfold tree_size; fold tree_size.
+    inversion H3.
+    - replace (d-2) with (-1) in H5 by lia; apply full_tree_equiv1 in H5.
+      pose proof full_tree_gt_0 _ _ H5; lia.
+    - assert (ls <> Leaf); [rewrite <- H4;discriminate|].
+      pose proof tree_compose_size_pop _ _ H3 H6.
+      rewrite <- H4 in H7.
+      replace (tree_size (tree_compose (skipn 1 (tree_to_partial_tree_pop (Node v0 ls0 rs0) (d - 1))) Leaf)) with (tree_size (Node v0 ls0 rs0) - 1) by lia.
+      lia.
+    - assert (ls <> Leaf); [rewrite <- H4;discriminate|].
+      pose proof tree_compose_size_pop _ _ H3 H6.
+      rewrite <- H4 in H7.
+      replace (tree_size (tree_compose (skipn 1 (tree_to_partial_tree_pop (Node v0 ls0 rs0) (d - 1))) Leaf)) with (tree_size (Node v0 ls0 rs0) - 1) by lia.
+      lia.
+  + pose proof complete_tree_pop_not_fullb _ _ H5.
+    replace (d-1-1) with (d-2) in H1 by lia; rewrite H1.
+    unfold tree_size; fold tree_size.
+    inversion H5.
+    - rewrite H2 in H3; inversion H3.
+      assert (tree_size (Node v ls rs) = 1); [simpl;rewrite <- H4; rewrite <- H7; tauto | ].
+      lia.
+      pose proof full_tree_gt_0 _ _ H6; lia.
+    - assert (rs <> Leaf); [rewrite <- H6;discriminate|].
+      pose proof tree_compose_size_pop _ _ H5 H7.
+      rewrite <- H6 in H8.
+      replace (tree_size (tree_compose (skipn 1 (tree_to_partial_tree_pop (Node v0 ls0 rs0) (d - 1))) Leaf)) with (tree_size (Node v0 ls0 rs0) - 1) by lia.
+      lia.
+    - assert (rs <> Leaf); [rewrite <- H6;discriminate|].
+      pose proof tree_compose_size_pop _ _ H5 H7.
+      rewrite <- H6 in H8.
+      replace (tree_size (tree_compose (skipn 1 (tree_to_partial_tree_pop (Node v0 ls0 rs0) (d - 1))) Leaf)) with (tree_size (Node v0 ls0 rs0) - 1) by lia.
+      lia.
+Qed.
+
 Lemma get_last_val_coincidence: forall d tr pt1 pt2,
   complete_tree_pop d tr ->
   tr <> Leaf ->
@@ -340,6 +536,189 @@ Proof.
     apply IHtr2; auto.
 Qed.
 
+Lemma list_nth_on_tree_decompose: forall l pt tr p n,
+  list_nth_on_tree l p tr ->
+  list_nth_on_partial_tree l n p pt ->
+  list_nth_on_tree l n (tree_compose pt tr).
+Proof.
+  intros.
+  revert l tr p n H H0.
+  induction pt; simpl; intros.
+  + inversion H0; [subst; auto | discriminate].
+  + inversion H0; [discriminate | subst].
+    injection H1; intros; subst.
+    destruct flg.
+    - eapply IHpt; [ | apply H6].
+      apply list_nth_on_tree_Node; try lia.
+      * replace (p / 2 * 2) with (p + -1) by lia; auto.
+      * rewrite <- H3; auto.
+    - eapply IHpt; [ | apply H6].
+      apply list_nth_on_tree_Node; try lia.
+      * replace (p / 2 * 2) with p by lia; auto.
+      * replace (p / 2 * 2) with p by lia; auto.
+Qed.
+
+Lemma list_nth_on_tree_update_less: forall l tr p n v,
+  list_nth_on_tree l p tr ->
+  0 <= n < p ->
+  list_nth_on_tree (upd_Znth n l v) p tr.
+Proof.
+  intros.
+  revert n v H0.
+  induction H; simpl; intros.
+  + apply list_nth_on_tree_Leaf.
+  + apply list_nth_on_tree_Node.
+    - rewrite upd_Znth_Zlength by lia; lia.
+    - rewrite upd_Znth_diff by lia; auto.
+    - apply IHlist_nth_on_tree1; lia.
+    - apply IHlist_nth_on_tree2; lia.  
+Qed.
+
+Lemma list_nth_on_partial_tree_update: forall l pt p n upd_pos v,
+  list_nth_on_partial_tree l n p pt ->
+  0 <= upd_pos < Zlength l -> upd_pos < n ->
+  list_nth_on_partial_tree (upd_Znth upd_pos l v) n p pt.
+Proof.
+  intros.
+  revert upd_pos v H0 H1.
+  induction H; simpl; subst; intros.
+  + apply nth_partial_tree_nil; auto.
+  + pose proof list_nth_on_partial_tree_no_less _ _ _ _ H4.
+    eapply nth_partial_tree_cons; eauto.
+    - rewrite upd_Znth_Zlength by lia.
+      lia. 
+    - rewrite upd_Znth_diff by lia; auto.
+    - apply list_nth_on_tree_update_less.
+      * auto.
+      * destruct flg; lia.
+Qed.
+
+Lemma list_nth_on_tree_impl_leaf: forall l tr p,
+  list_nth_on_tree l p tr ->
+  p >= Zlength l ->
+  tr = Leaf.
+Proof.
+  intros.
+  inversion H; [auto | lia].
+Qed.
+
+
+Lemma list_nth_on_tree_coin: forall tr l n len d,
+  complete_tree_pop d tr ->
+  list_nth_on_tree l n tr ->
+  len >= last_index d n tr ->
+  n < len <= Zlength l ->
+  list_nth_on_tree (firstn (Z.to_nat len) l) n tr.
+Proof.
+  intros tr.
+  induction tr; simpl; intros.
+  + apply list_nth_on_tree_Leaf.
+  + inversion H; subst.
+    - rewrite full_tree_equiv1 in H7.
+      rewrite H7 in H1.
+      inversion H0; subst.
+      apply list_nth_on_tree_Node.
+      * rewrite Zlength_firstn; lia.
+      * rewrite Znth_firstn; [auto | lia].
+      * assert (n * 2 >= len \/ n * 2 < len) by lia.
+        destruct H3.
+        ++ pose proof list_nth_on_tree_impl_leaf.
+Admitted.
+
+Lemma list_on_tree_coincidence_r: forall v ls rs l p d,
+  list_nth_on_tree l p (Node v ls rs) ->
+  complete_tree_pop d (Node v ls rs) ->
+  full_tree_b (d - 2) rs = true ->
+  list_nth_on_tree (firstn (Z.to_nat (Zlength l - 1)) l) (p * 2 + 1) rs.
+Proof.
+  intros.
+  revert l p d v ls H H1 H0.
+  induction rs; simpl; intros.
+  + apply list_nth_on_tree_Leaf.
+  + inversion H; subst.
+    inversion H8; subst.
+    apply list_nth_on_tree_Node.
+    - rewrite Zlength_firstn by lia.
+      
+Admitted.
+
+Lemma list_on_tree_coincidence_l: forall v ls rs l p d,
+  list_nth_on_tree l p (Node v ls rs) ->
+  complete_tree_pop d (Node v ls rs) ->
+  full_tree_b (d - 2) rs = false ->
+  list_nth_on_tree (firstn (Z.to_nat (Zlength l - 1)) l) (p * 2) ls.
+Proof.
+  intros.
+Admitted.
+
+Lemma list_on_tree_to_pt_pop: forall l tr pt d1 d2 n p,
+  tr <> Leaf ->
+  list_nth_on_tree l p tr ->
+  list_nth_on_partial_tree (firstn (Z.to_nat (Zlength l - 1)) l) n p pt ->
+  complete_tree_pop d1 (tree_compose pt tr) ->
+  complete_tree_pop d2 tr ->
+  list_nth_on_partial_tree (firstn (Z.to_nat (Zlength l - 1)) l) n (last_index d2 p tr) (skipn 1 (tree_to_partial_tree_pop_fix pt tr d2)).
+Proof.
+  intros.
+  revert l d1 d2 n p pt H0 H1 H2 H3.
+  induction tr; simpl; intros.
+  + contradiction.
+  + inversion H3; subst.
+    - rewrite full_tree_equiv1 in H8.
+      rewrite H8.
+      fold (skipn 1 (tree_to_partial_tree_pop_fix ((false, v, tr2) :: pt) tr1
+      (d2 - 1))).
+      destruct (classic (tr1 = Leaf)).
+      1: {
+        subst.
+        inversion H6.
+        rewrite <- full_tree_equiv1 in H8.
+        pose proof full_tree_nonneg _ _ H8.
+        lia.
+      }
+      eapply IHtr1; eauto; inversion H0; subst.
+      * auto.
+      * inversion H12.
+        1: { rewrite H5 in H4; contradiction. }
+        eapply nth_partial_tree_cons; eauto.
+        ++ rewrite Z.div_mul by lia.
+           rewrite Zlength_firstn.
+           lia.
+        ++ rewrite Z.div_mul by lia; lia.
+        ++ rewrite Z.div_mul by lia.
+           rewrite Znth_firstn by lia.
+           auto.
+        ++ simpl.
+           eapply list_on_tree_coincidence_r; eauto.
+        ++ rewrite Z.div_mul by lia; auto.  
+    - pose proof complete_tree_pop_not_fullb _ _ H8.
+      replace (d2 - 1 - 1) with (d2 - 2) in H4 by lia.
+      rewrite H4.
+      inversion H0; subst.
+      destruct (classic (tr2 = Leaf)).
+      1: {
+        subst; simpl.
+        rewrite Odd_Div2 by lia; auto.
+      }
+      fold (skipn 1 ( tree_to_partial_tree_pop_fix ((true, Znth p l, tr1) :: pt) tr2
+      (d2 - 1))).
+      eapply IHtr2; eauto.
+      inversion H13.
+      1: { rewrite H7 in H5; contradiction. }
+      eapply nth_partial_tree_cons; eauto.
+      * rewrite Odd_Div2 by lia.
+        rewrite Zlength_firstn.
+        lia.
+      * rewrite Odd_Div2 by lia; lia.
+      * rewrite Odd_Div2 by lia.
+        rewrite Znth_firstn by lia.
+        auto.
+      * simpl.
+        replace (p * 2 + 1 + -1) with (p * 2) by lia.
+        eapply list_on_tree_coincidence_l; eauto.
+      * rewrite Odd_Div2 by lia; auto.    
+Qed.
+
 Lemma list_on_tree_impl_state: forall (l: list Z) (ls rs: tree) (v: Z),
   Zlength l > 2 -> list_on_tree l (Node v ls rs) ->
   exists d, list_on_tree_state (firstn (Z.to_nat (Zlength l - 1)) (upd_Znth 1 l (Znth (Zlength l - 1) l)), 1) (nil, tree_cut_last ls rs d) /\  complete_tree_pop d (Node v ls rs).
@@ -362,6 +741,14 @@ Proof.
     inversion H2; subst.
     + rewrite full_tree_equiv1 in H7.
       rewrite H7.
+      assert (Zlength l - 1 = last_index d 1 (Node v ls rs)). {
+        rewrite tree_last_index_size by auto; lia.
+      }
+      assert (ls <> Leaf). {
+        rewrite <- full_tree_equiv1 in H7.
+        pose proof full_tree_nonneg _ _ H7.
+        eapply complete_tree_pop_not_leaf; eauto; lia.
+      }
       apply list_nth_on_tree_Node.
       - rewrite Zlength_firstn.
         rewrite upd_Znth_Zlength by lia.
@@ -369,14 +756,6 @@ Proof.
       - rewrite Znth_firstn by lia.
         rewrite upd_Znth_same by lia.
         unfold tree_to_partial_tree_pop.
-        assert (Zlength l - 1 = last_index d 1 (Node v ls rs)). {
-          rewrite tree_last_index_size by auto; lia.
-        }
-        assert (ls <> Leaf). {
-          rewrite <- full_tree_equiv1 in H7.
-          pose proof full_tree_nonneg _ _ H7.
-          eapply complete_tree_pop_not_leaf; eauto; lia.
-        }
         rewrite get_last_val_coincidence with (pt2 := (false, v, rs) :: nil); auto.
         replace (tree_to_partial_tree_pop_fix [(false, v, rs)] ls (d - 1)) with (tree_to_partial_tree_pop_fix nil (Node v ls rs) d).
         2: { simpl; rewrite H7; auto. }
@@ -391,7 +770,19 @@ Proof.
           -- simpl in H1; lia. 
           -- apply complete_tree_equality.
              exists d; auto.
-      - admit.
+      - apply list_nth_on_tree_decompose with (p := last_index d 1 (Node v ls rs)).
+        1: {apply list_nth_on_tree_Leaf. }
+        unfold tree_to_partial_tree_pop.
+        simpl.
+        rewrite H7.
+        fold (skipn 1 (tree_to_partial_tree_pop_fix [] ls (d - 1))).
+        rewrite <- sublist_firstn.
+        rewrite sublist_upd_Znth_lr by lia.
+        rewrite sublist_firstn.
+        apply list_nth_on_partial_tree_update; [ | rewrite Zlength_firstn by lia; lia | lia].
+        eapply list_on_tree_to_pt_pop; eauto.
+        * inversion H0; replace (1 * 2) with 2 in H12 by lia; auto.
+        * apply nth_partial_tree_nil; auto.   
       - admit.
     + pose proof complete_tree_pop_not_fullb _ _ H7.
       replace (d - 1 - 1) with (d - 2) in H3 by lia.
@@ -411,6 +802,7 @@ Proof.
             2: { pose proof full_tree_nonneg _ _ H9; lia. }
             subst.
             simpl in H1; lia.
+          + give_up. 
         }
         assert (Zlength l - 1 = last_index d 1 (Node v ls rs)). {
           rewrite tree_last_index_size by auto; lia.
@@ -432,22 +824,125 @@ Proof.
       - admit.
       - admit. 
   } 
-  
-Admitted.
 
-Lemma tree_not_emp: forall (t: tree),
-  tree_size t >= 1 -> exists v ls rs, t = Node v ls rs.
-Proof.
-  intros.
-  destruct t.
-  + simpl in H; lia. 
-  + exists v, t1, t2; reflexivity. 
-Qed.
+Admitted.
 
 Lemma MaxHeap_tree_down_state: forall (ls rs: tree) (d v: Z),
-  MaxHeap (Node v ls rs) -> complete_tree_pop d (Node v ls rs) -> MaxHeap_tree_down ([], tree_cut_last ls rs d).
+  tree_size (Node v ls rs) >= 2 -> MaxHeap (Node v ls rs) -> complete_tree_pop d (Node v ls rs) ->
+  MaxHeap_tree_down ([], tree_cut_last ls rs d).
 Proof.
-Admitted.
+  intros.
+  unfold MaxHeap_tree_down; simpl.
+  split; [apply MaxHeap_partial_tree_v_nil; reflexivity|].
+  split.
+  + unfold tree_cut_last.
+    inversion H0; [discriminate|].
+    unfold MaxHeap_no_rt.
+    inversion H1; subst.
+    - apply full_tree_equiv1 in H11.
+      rewrite H11.
+      exists (get_last_val (tree_to_partial_tree_pop ls (d - 1))), (tree_compose (skipn 1 (tree_to_partial_tree_pop ls (d - 1))) Leaf), rs.
+      injection H2; intros; subst.
+      split; [tauto|].
+      split; [|tauto].
+      apply tree_compose_MaxHeap; [apply MaxHeap_Leaf; tauto|left].
+      split; [reflexivity|].
+      apply MaxHeap_tree_partial_tree_skip.
+      unfold tree_to_partial_tree_pop.
+      apply MaxHeap_tree_partial_hold; try tauto; [|unfold MaxHeap_partial_tree; tauto].
+      destruct H5; [left;tauto|right].
+      apply MaxHeap_partial_tree_v_nil.
+      reflexivity.
+    - pose proof complete_tree_pop_not_fullb _ _ H11.
+      replace (d-1-1) with (d-2) in H7 by lia.
+      rewrite H7.
+      exists (get_last_val (tree_to_partial_tree_pop rs (d - 1))), ls, (tree_compose (skipn 1 (tree_to_partial_tree_pop rs (d - 1))) Leaf).
+      injection H2; intros; subst.
+      split; [tauto|].
+      split; [tauto|].
+      apply tree_compose_MaxHeap; [apply MaxHeap_Leaf; tauto|left].
+      split; [reflexivity|].
+      apply MaxHeap_tree_partial_tree_skip.
+      unfold tree_to_partial_tree_pop.
+      apply MaxHeap_tree_partial_hold; try tauto; [|unfold MaxHeap_partial_tree; tauto].
+      destruct H6; [left;tauto|right].
+      apply MaxHeap_partial_tree_v_nil.
+      reflexivity.
+  + pose proof tree_cut_last_size ls rs v d H H1.
+    simpl in H.
+    pose proof tree_not_emp (tree_cut_last ls rs d) ltac:(lia).
+    destruct H3 as [v0 [ls0 [rs0]]].
+    exists v0, ls0, rs0.
+    split; [tauto|].
+    split; right; apply MaxHeap_partial_tree_v_nil; tauto.
+Qed.
+
+Lemma complete_tree_pop_holds: forall (t: tree)(d: Z), 
+   t <> Leaf -> complete_tree_pop d t -> complete_tree_push d (tree_compose (skipn 1%nat (tree_to_partial_tree_pop t d)) Leaf).
+Proof.
+  intros.
+  induction H0.
+  + tauto.
+  + unfold tree_to_partial_tree_pop.
+    unfold tree_to_partial_tree_pop_fix; fold tree_to_partial_tree_pop_fix.
+    apply full_tree_equiv1 in H1; rewrite H1.
+    apply full_tree_equiv1 in H1.
+    destruct ls.
+    - inversion H0.
+      replace (dep-2) with (-1) in H1 by lia.
+      pose proof full_tree_gt_0 _ _ H1; lia.
+    - replace ((false, v, rs) :: nil) with (nil ++ [(false, v, rs)]); [|  rewrite app_nil_l; tauto].
+      rewrite tree_to_partial_tree_pop_get.
+      pose proof tree_to_partial_tree_len (Node v0 ls1 ls2) (dep - 1) ltac:(discriminate).
+      replace 1%nat with (Z.to_nat 1) by lia.
+      rewrite Zskipn_app1; [|unfold tree_to_partial_tree_pop in H2; lia].
+      rewrite tree_compose_append.
+      apply complete_tree_push_right_full; [|tauto].
+      apply IHcomplete_tree_pop; discriminate.
+  + unfold tree_to_partial_tree_pop.
+    unfold tree_to_partial_tree_pop_fix; fold tree_to_partial_tree_pop_fix.
+    pose proof complete_tree_pop_not_fullb _ _ H1.
+    replace (dep-1-1) with (dep-2) in H2 by lia; rewrite H2.
+    destruct rs.
+    - inversion H1.
+      simpl.
+      replace dep with 1 by lia.
+      apply complete_tree_push_Leaf; lia.
+    - replace ((true, v, ls) :: nil) with (nil ++ [(true, v, ls)]); [|  rewrite app_nil_l; tauto].
+      rewrite tree_to_partial_tree_pop_get.
+      pose proof tree_to_partial_tree_len (Node v0 rs1 rs2) (dep - 1) ltac:(discriminate).
+      replace 1%nat with (Z.to_nat 1) by lia.
+      rewrite Zskipn_app1; [|unfold tree_to_partial_tree_pop in H3; lia].
+      rewrite tree_compose_append.
+      apply complete_tree_push_left_full; [tauto|].
+      apply IHcomplete_tree_pop; discriminate.
+Qed. 
+
+Lemma complete_tree_pop_holds_all: forall (ls rs: tree)(d v: Z), 
+   complete_tree_pop d (Node v ls rs) -> tree_size (Node v ls rs) >= 2 -> complete_tree_push d (tree_cut_last ls rs d).
+Proof.
+  intros.
+  rename H0 into HH.
+  unfold tree_cut_last.
+  inversion H; subst.
+  + apply full_tree_equiv1 in H4; rewrite H4.
+    apply full_tree_equiv1 in H4.
+    apply complete_tree_push_right_full; [|tauto].
+    apply complete_tree_pop_holds; [|tauto].
+    destruct ls; [|discriminate].
+    inversion H2; replace (d-2) with (-1) in H4 by lia.
+    pose proof full_tree_gt_0 _ _ H4; lia.
+  + pose proof complete_tree_pop_not_fullb _ _ H4.
+    replace (d-1-1) with (d-2) in H0 by lia; rewrite H0.
+    apply complete_tree_push_left_full; [tauto|].
+    apply complete_tree_pop_holds; [|tauto].
+    destruct rs; [|discriminate].
+    inversion H4.
+    rewrite H1 in H2.
+    inversion H2.
+    - rewrite <- H5 in HH; simpl in HH; lia.
+    - pose proof full_tree_gt_0 _ _ H5; lia.
+Qed.
 
 Lemma Pop_tree_list_rel: forall (l l': list Z) (t: tree),
   list_on_tree l t -> heap_pop l l' -> MaxHeap t ->
@@ -481,11 +976,20 @@ Proof.
     destruct H4.
     assert (Zlength (fst (firstn (Z.to_nat (Zlength l - 1))
           (upd_Znth 1 l (Znth (Zlength l - 1) l)), 1)) >= 2). {
-      give_up.
+      simpl.
+      rewrite Zlength_firstn.
+      replace (Z.max 0 (Zlength l -1)) with (Zlength l -1) by lia.
+      rewrite upd_Znth_Zlength; [|lia].
+      lia.
     }
     pose proof Down_tree_list_rel _ _ _ H6 H4 H2.
     subst.
-    pose proof MaxHeap_tree_down_state _ _ _ _ H1 H5.
+    assert (tree_size (Node v ls rs) >= 2). {
+      destruct H, H3.
+      rewrite H3; lia.
+    }
+    rename H3 into HH.
+    pose proof MaxHeap_tree_down_state _ _ _ _ HH H1 H5.
     specialize (H7 H3).
     destruct H7 as [t'].
     destruct H7, H8.
@@ -495,6 +999,8 @@ Proof.
     split; [tauto|].
     split; [tauto|].
     unfold tree_pop; right.
+    destruct H, H11.
+    split; [lia|].
     exists v, ls, rs, t', d.
     tauto.
-Admitted.
+Qed.
