heap/tree_set.v
@@ -1,0 +1,574 @@
+Require Import FloydSeq.proofauto.
+(* Require Import cprogs.heap.program. *)
+Require Import Notations Logic Datatypes.
+From Coq Require Import String List ZArith. 
+From compcert Require Import Coqlib Integers Floats AST Ctypes Cop Clight Clightdefs.
+Require Import Coq.Logic.Classical_Pred_Type.
+Require Import Classical_Prop.
+Require Export SetsClass.SetsClass.
+
+Require Import Coq.micromega.Psatz.
+Local Open Scope string.
+Local Open Scope nat_scope.
+Local Open Scope Z_scope.
+Local Open Scope list_scope.
+Require Import cprogs.heap.list_relation.
+Require Import cprogs.heap.definitions.
+Require Import cprogs.heap.tree_list.
+Require Import cprogs.heap.tree_down.
+Require Import cprogs.heap.tree_push.
+Require Import cprogs.heap.tree_up.
+Require Import cprogs.heap.tree_pop.
+Local Open Scope sets.
+Local Open Scope logic.
+
+Definition SetZ: Type := Z -> Prop.
+
+Definition Singleton (k: Z): SetZ:=
+  fun x => x = k.
+
+Fixpoint SetOf_tree(t: tree): SetZ:=
+  match t with
+    | Leaf => ∅
+    | Node v ls rs => 
+        Singleton v ∪ (SetOf_tree ls) ∪ (SetOf_tree rs)
+  end.
+
+Fixpoint SetOf_partial_tree(lt: partial_tree): SetZ:=
+  match lt with
+    | nil => ∅
+    | (flg, v, tr) :: lt0 => Singleton v ∪ SetOf_tree tr ∪ SetOf_partial_tree lt0
+  end.
+
+Definition tree_set_rel(t: tree) (s: SetZ): Prop :=
+  forall x, SetOf_tree t x <-> s x.
+
+Definition SetOf_tree_state(t: tree_state): SetZ:=
+  SetOf_partial_tree (fst t) ∪ SetOf_tree (snd t).
+
+Lemma Set_eq_on_tree: forall (t: tree),
+  tree_set_rel t (SetOf_tree t).
+Proof.
+  intros.
+  unfold tree_set_rel.
+  intros x.
+  reflexivity.
+Qed.
+
+Lemma SetSplit: forall (ls rs: tree) (s: SetZ) (v: Z),
+  tree_set_rel (Node v ls rs) s -> 
+  exists L R, tree_set_rel ls L /\ tree_set_rel rs R /\ s == Singleton v ∪ L ∪ R.
+Proof.
+  intros.
+  exists (SetOf_tree ls), (SetOf_tree rs).
+  split; [apply Set_eq_on_tree|].
+  split; [apply Set_eq_on_tree|].
+  unfold_RELS_tac; intros.
+  split.
+  + unfold tree_set_rel in H.
+    apply H.
+  + unfold tree_set_rel in H.
+    apply H.
+Qed.
+
+Lemma tree_compose_set_union: forall (lt: partial_tree) (t: tree),
+  SetOf_tree (tree_compose lt t) == SetOf_tree t ∪ SetOf_partial_tree lt.
+Proof.
+  intros.
+  revert t.
+  induction lt; intros.
+  + simpl.
+    rewrite Sets_union_empty.
+    reflexivity.
+  + destruct a as [[flg val] tr].
+    simpl.
+    destruct flg.
+    - rewrite IHlt.
+      unfold SetOf_tree; fold SetOf_tree.
+      unfold_RELS_tac.
+      intros.
+      tauto.
+    - rewrite IHlt.
+      unfold SetOf_tree; fold SetOf_tree.
+      unfold_RELS_tac.
+      intros.
+      tauto.
+Qed.
+
+Lemma tree_to_partial_tree_set_eq: forall (t: tree) (lt: partial_tree) (d: Z),
+  complete_tree_push d t -> SetOf_tree t ∪ SetOf_partial_tree lt == SetOf_partial_tree (tree_to_partial_tree_fix lt t d).
+Proof.
+  intros.
+  revert lt.
+  induction H; intros.
+  + simpl.
+    rewrite Sets_empty_union.
+    reflexivity.
+  + simpl.
+    apply full_tree_equiv1 in H.
+    rewrite H.
+    rewrite <- IHcomplete_tree_push.
+    simpl.
+    unfold_RELS_tac; intros; tauto.
+  + simpl.
+    pose proof complete_tree_push_not_fullb _ _ H.
+    rewrite H1.
+    rewrite <- IHcomplete_tree_push.
+    simpl.
+    unfold_RELS_tac; intros; tauto.
+Qed.
+
+Lemma tree_up_succeed_Set_eq: forall (t t': tree_state),
+  tree_up_succeed t t' -> SetOf_tree_state t == SetOf_tree_state t'.
+Proof.
+  intros.
+  unfold tree_up_succeed in H.
+  destruct H as [t3 [l']].
+  destruct H, H0.
+  destruct H1.
+  destruct H1 as [v [ls [rs]]].
+  destruct H1.
+  unfold SetOf_tree_state.
+  rewrite <- H; rewrite <- H0.
+  destruct t3 as [[flg val] tr].
+  unfold swap_up_and_combine in H1; simpl in H1.
+  destruct flg.
+  + rewrite H3.
+    rewrite <- H1.
+    simpl.
+    unfold_RELS_tac; intros; tauto.
+  + rewrite H3.
+    rewrite <- H1.
+    simpl.
+    unfold_RELS_tac; intros; tauto.
+Qed.
+
+Lemma heap_tree_up_Set_eq: forall (t t': tree_state),
+  heap_tree_up t t' -> SetOf_tree_state t == SetOf_tree_state t'.
+Proof.
+  intros.
+  unfold heap_tree_up in H.
+  revert H; unfold_RELS_tac; intros.
+  destruct H as [t0].
+  destruct H.
+  unfold tree_up_fail in H0.
+  revert H0; simpl; intros.
+  destruct H0; subst.
+  induction_1n H.
+  + reflexivity.
+  + pose proof tree_up_succeed_Set_eq _ _ H1.
+    revert H2; unfold_RELS_tac; intros.
+    specialize (H2 a).
+    rewrite H2.
+    apply IHrt.
+    tauto.
+Qed.
+
+Lemma Push_to_Set: forall (t t': tree) (s: SetZ) (v: Z),
+  tree_set_rel t s -> (exists d, complete_tree_push d t) -> tree_push t v t' -> MaxHeap t ->
+  exists s', tree_set_rel t' s' /\ s' == s ∪ Singleton v.
+Proof.
+  intros.
+  clear H2.
+  destruct H0 as [d].
+  unfold tree_push in H1.
+  destruct H1 as [ts [dep1 [dep2]]].
+  exists (SetOf_tree t').
+  split.
+  + unfold tree_set_rel.
+    tauto.
+  + destruct H1, H2, H3.
+    pose proof heap_tree_up_Set_eq _ _ H1.
+    unfold tree_to_partial_tree in H5.
+    pose proof tree_to_partial_tree_set_eq _ nil _ H2.
+    simpl in H6.
+    unfold SetOf_tree_state in H5; simpl in H5.
+    rewrite <- H6 in H5.
+    pose proof tree_compose_set_union (fst ts) (snd ts).
+    rewrite <- H3 in H7.
+    rewrite H7.
+    assert (SetOf_tree t ∪ ∅ ∪ (Singleton v ∪ ∅ ∪ ∅) == s ∪ Singleton v). {
+      rewrite ! Sets_union_empty.
+      unfold tree_set_rel in H.
+      assert (SetOf_tree t == s). {
+        unfold_RELS_tac; apply H.
+      }
+      rewrite H8.
+      reflexivity.
+    }
+    rewrite H8 in H5.
+    rewrite H5.
+    unfold_RELS_tac; tauto.
+Qed.
+
+Definition MaxSetElement(x: Z) (s: SetZ): Prop := 
+  s x /\ (forall v, s v -> v <= x).
+
+Lemma tree_max_set: forall (t: tree) (s: SetZ),
+  tree_set_rel t s -> MaxHeap t -> (exists d, complete_tree_push d t) -> 
+  (t = Leaf \/ (exists v ls rs, t = Node v ls rs /\ MaxSetElement v s)).
+Proof.
+  intros.
+  clear H1.
+  revert s H.
+  induction H0.
+  + left; tauto.
+  + right.
+    rewrite H; simpl.
+    rewrite H in H2.
+    pose proof SetSplit _ _ _ _ H2.
+    destruct H3 as [L [R]].
+    destruct H3, H4.
+    exists v, ls, rs.
+    split; [reflexivity|].
+    revert H5; unfold_RELS_tac; intros.
+    split.
+    - rewrite H5.
+      left; left.
+      unfold Singleton.
+      reflexivity.
+    - intros.
+      apply H5 in H6.
+      destruct H6.
+      * destruct H6.
+        unfold Singleton in H6.
+        lia.
+        specialize (IHMaxHeap1 L H3).
+        rename IHMaxHeap1 into HH.
+        destruct HH.
+        ++ rewrite H7 in H3.
+           unfold tree_set_rel in H3.
+           simpl in H3.
+           apply (H3 v0) in H6.
+           tauto.
+        ++ destruct H7 as [val [lls [rrs]]].
+           destruct H7, H8.
+           specialize (H9 v0 H6).
+           rewrite H7 in H0.
+           destruct H0; [discriminate|].
+           unfold get_tree_val in H0.
+           lia.
+      * specialize (IHMaxHeap2 R H4).
+        rename IHMaxHeap2 into HH.
+        destruct HH.
+        ++ rewrite H7 in H4.
+           unfold tree_set_rel in H4.
+           simpl in H4.
+           apply (H4 v0) in H6.
+           tauto.
+        ++ destruct H7 as [val [lls [rrs]]].
+           destruct H7, H8.
+           specialize (H9 v0 H6).
+           rewrite H7 in H1.
+           destruct H1; [discriminate|].
+           unfold get_tree_val in H1.
+           lia.
+Qed.
+
+Lemma get_last_val_len_gt_1: forall (lt: partial_tree) (flg: bool) (v: Z) (t: tree),
+  1 <= Zlength lt -> get_last_val (lt ++ [(flg,v,t)]) = get_last_val lt.
+Proof.
+  intros.
+  destruct lt.
+  + replace (Zlength []) with 0 in H by tauto.
+    lia.
+  + replace (p :: lt) with ([p] ++ lt) by reflexivity.
+    rewrite <- app_assoc.
+    simpl; tauto. 
+Qed.
+
+Lemma get_skipn_len_gt_1: forall (lt: partial_tree) (flg: bool) (v: Z) (t: tree),
+  1 <= Zlength lt -> SetOf_partial_tree (skipn 1 (lt ++ [(flg,v,t)])) == SetOf_partial_tree (skipn 1 lt) ∪ (SetOf_tree t) ∪ (Singleton v).
+Proof.
+  intros.
+  induction lt.
+  + replace (Zlength []) with 0 in H by tauto.
+    lia.
+  + simpl. 
+    destruct lt.
+    - simpl; unfold_RELS_tac; tauto.
+    - destruct p as [[flg0 val] tr].
+      simpl.
+      simpl in IHlt.
+      rewrite IHlt.
+      * unfold_RELS_tac; tauto.
+      * rewrite Zlength_cons.
+        pose proof initial_world.zlength_nonneg _ lt.
+        lia.
+Qed.
+
+Lemma partial_tree_splt2: forall (lt1 lt2: partial_tree),
+  SetOf_partial_tree (lt1 ++ lt2) == SetOf_partial_tree lt1 ∪ SetOf_partial_tree lt2.
+Proof.
+  intros.
+  induction lt1.
+  + simpl; unfold_RELS_tac; tauto.
+  + destruct a as [[flg1 val] tr].
+    simpl.
+    rewrite IHlt1. 
+    unfold_RELS_tac; tauto.
+Qed.
+
+Lemma partial_tree_split: forall (t: tree) (d: Z),
+  t <> Leaf -> complete_tree_pop d t -> Singleton (get_last_val (tree_to_partial_tree_pop t d)) ∪ (SetOf_partial_tree (skipn 1 (tree_to_partial_tree_pop t d))) == SetOf_tree t.
+Proof.
+  intros.
+  induction H0.
+  + tauto.
+  + unfold tree_to_partial_tree_pop.
+    unfold tree_to_partial_tree_pop_fix;
+    fold tree_to_partial_tree_pop_fix.
+    apply full_tree_equiv1 in H1; rewrite ! H1.
+    apply full_tree_equiv1 in H1.
+    destruct ls.
+    - simpl; inversion H0.
+      replace (dep-2) with (-1) in H1 by lia.
+      pose proof full_tree_gt_0 _ _ H1; lia.
+    - pose proof tree_to_partial_tree_len (Node v0 ls1 ls2) (dep-1).
+      replace ((false, v, rs) :: nil) with (nil ++ [(false, v, rs)]); [|rewrite app_nil_l; tauto].
+      rewrite tree_to_partial_tree_pop_get.
+      unfold tree_to_partial_tree_pop in H2.
+      replace 1%nat with (Z.to_nat 1) by lia.
+      rewrite Zskipn_app1; [|apply H2; discriminate].
+      rewrite get_last_val_len_gt_1; [|apply H2; discriminate].
+      replace (Z.to_nat 1) with 1%nat by lia.
+      rewrite partial_tree_splt2.
+      unfold tree_to_partial_tree_pop in IHcomplete_tree_pop.
+      rewrite <- Sets_union_assoc.
+      rewrite IHcomplete_tree_pop; [|discriminate].
+      simpl; unfold_RELS_tac; tauto.
+  + unfold tree_to_partial_tree_pop.
+    unfold tree_to_partial_tree_pop_fix;
+    fold tree_to_partial_tree_pop_fix.
+    pose proof complete_tree_pop_not_fullb _ _ H1.
+    replace (dep-1-1) with (dep-2) in H2 by lia.
+    rewrite H2.
+    destruct rs.
+    - inversion H1.
+      rewrite H3 in H0.
+      inversion H0.
+      simpl; unfold_RELS_tac; tauto.
+      pose proof full_tree_gt_0 _ _ H5; lia.
+    - pose proof tree_to_partial_tree_len (Node v0 rs1 rs2) (dep-1).
+      replace ((true, v, ls) :: nil) with (nil ++ [(true, v, ls)]); [|rewrite app_nil_l; tauto].
+      rewrite tree_to_partial_tree_pop_get.
+      unfold tree_to_partial_tree_pop in H3.
+      replace 1%nat with (Z.to_nat 1) by lia.
+      rewrite Zskipn_app1; [|apply H3; discriminate].
+      rewrite get_last_val_len_gt_1; [|apply H3; discriminate].
+      replace (Z.to_nat 1) with 1%nat by lia.
+      rewrite partial_tree_splt2.
+      unfold tree_to_partial_tree_pop in IHcomplete_tree_pop.
+      rewrite <- Sets_union_assoc.
+      rewrite IHcomplete_tree_pop; [|discriminate].
+      simpl; unfold_RELS_tac; tauto.
+Qed.
+
+Lemma tree_to_partial_tree_pop_set_eq: forall (t: tree) (lt: partial_tree) (d: Z),
+  complete_tree_pop d t -> SetOf_tree t ∪ SetOf_partial_tree lt == SetOf_partial_tree (tree_to_partial_tree_pop_fix lt t d).
+Proof.
+  intros.
+  revert lt.
+  induction H; intros.
+  + simpl.
+    rewrite Sets_empty_union.
+    reflexivity.
+  + simpl.
+    apply full_tree_equiv1 in H0.
+    rewrite H0.
+    rewrite <- IHcomplete_tree_pop.
+    simpl.
+    unfold_RELS_tac; intros; tauto.
+  + simpl.
+    pose proof complete_tree_pop_not_fullb _ _ H0.
+    replace (dep-1-1) with (dep-2) in H1 by lia.
+    rewrite H1.
+    rewrite <- IHcomplete_tree_pop.
+    simpl.
+    unfold_RELS_tac; intros; tauto.
+Qed.
+
+Lemma tree_cut_last_set: forall (ls rs: tree) (d v: Z),
+  tree_size (Node v ls rs) >= 2 -> complete_tree_pop d (Node v ls rs) -> (SetOf_tree (tree_cut_last ls rs d)) ∪ Singleton v == SetOf_tree (Node v ls rs).
+Proof.
+  intros.
+  inversion H0; subst.
+  + unfold tree_cut_last.
+    apply full_tree_equiv1 in H5.
+    rewrite H5.
+    unfold SetOf_tree; fold SetOf_tree.
+    rewrite tree_compose_set_union. 
+    inversion H3.
+    - replace (d-2) with (-1) in H5 by lia.
+      apply full_tree_equiv1 in H5.
+      pose proof full_tree_gt_0 _ _ H5; lia.
+    - unfold tree_to_partial_tree_pop.
+      simpl SetOf_tree.
+      rewrite Sets_empty_union.
+      rewrite partial_tree_split.
+      * simpl; unfold_RELS_tac; tauto.
+      * discriminate.
+      * rewrite H4; tauto.
+    - unfold tree_to_partial_tree_pop.
+      simpl SetOf_tree.
+      rewrite Sets_empty_union.
+      rewrite partial_tree_split.
+      * simpl; unfold_RELS_tac; tauto.
+      * discriminate.
+      * rewrite H4; tauto.
+  + unfold tree_cut_last.
+    pose proof complete_tree_pop_not_fullb _ _ H5.
+    replace (d-1-1) with (d-2) in H1 by lia.
+    rewrite H1.
+    unfold SetOf_tree; fold SetOf_tree.
+    rewrite tree_compose_set_union. 
+    inversion H5.
+    - rewrite H2 in H3.
+      inversion H3.
+      * simpl in H.
+        rewrite <- H4 in H.
+        rewrite <- H7 in H.
+        simpl in H; lia.
+      * pose proof full_tree_gt_0 _ _ H7; lia.
+    - unfold tree_to_partial_tree_pop.
+      rewrite ! Sets_union_assoc.
+      assert( (Singleton (get_last_val (tree_to_partial_tree_pop_fix []%list (Node v0 ls0 rs0) (d - 1))) ∪ (SetOf_tree ls ∪ (SetOf_tree Leaf ∪ (SetOf_partial_tree (skipn 1 (tree_to_partial_tree_pop_fix []%list (Node v0 ls0 rs0) (d - 1))) ∪ Singleton v)))) == ((Singleton (get_last_val (tree_to_partial_tree_pop_fix []%list (Node v0 ls0 rs0) (d - 1))) ∪ SetOf_partial_tree (skipn 1 (tree_to_partial_tree_pop_fix []%list (Node v0 ls0 rs0) (d - 1))) )∪(SetOf_tree Leaf ∪ Singleton v ∪ SetOf_tree ls)) ). {
+        unfold_RELS_tac.
+        tauto.
+      }
+      rewrite H7.
+      rewrite partial_tree_split.
+      * simpl; unfold_RELS_tac; tauto.
+      * discriminate.
+      * rewrite H6; tauto.
+    - unfold tree_to_partial_tree_pop.
+      rewrite ! Sets_union_assoc.
+      assert( (Singleton (get_last_val (tree_to_partial_tree_pop_fix []%list (Node v0 ls0 rs0) (d - 1))) ∪ (SetOf_tree ls ∪ (SetOf_tree Leaf ∪ (SetOf_partial_tree (skipn 1 (tree_to_partial_tree_pop_fix []%list (Node v0 ls0 rs0) (d - 1))) ∪ Singleton v)))) == ((Singleton (get_last_val (tree_to_partial_tree_pop_fix []%list (Node v0 ls0 rs0) (d - 1))) ∪ SetOf_partial_tree (skipn 1 (tree_to_partial_tree_pop_fix []%list (Node v0 ls0 rs0) (d - 1))) )∪(SetOf_tree Leaf ∪ Singleton v ∪ SetOf_tree ls)) ). {
+        unfold_RELS_tac.
+        tauto.
+      }
+      rewrite H7.
+      rewrite partial_tree_split.
+      * simpl; unfold_RELS_tac; tauto.
+      * discriminate.
+      * rewrite H6; tauto.
+Qed.
+
+Lemma tree_down_succeed_Set_eq: forall (t t': tree_state),
+  tree_down_succeed t t' -> SetOf_tree_state t == SetOf_tree_state t'.
+Proof.
+  intros.
+  unfold tree_down_succeed in H.
+  destruct H.
+  destruct x as [[flg v] tr].
+  destruct H.
+  destruct H0 as [v0 [ls [rs]]].
+  destruct H0.
+  destruct H1.
+  + destruct H1, H2.
+    unfold swap_down_left in H3.
+    destruct H3 as [vl [lls [lrs]]].
+    destruct H3, H4.
+    injection H5; intros; subst.
+    unfold SetOf_tree_state.
+    rewrite <- H.
+    rewrite H0, H4.
+    simpl.
+    unfold_RELS_tac; tauto.
+  + destruct H1.
+    - destruct H1, H2.
+      unfold swap_down_right in H3.
+      destruct H3 as [vr [rls [rrs]]].
+      destruct H3, H4.
+      injection H5; intros; subst.
+      unfold SetOf_tree_state.
+      rewrite <- H.
+      rewrite H0, H4.
+      simpl.
+      unfold_RELS_tac; tauto.
+    - destruct H1, H2, H3, H3.
+      * unfold swap_down_right in H4.
+        destruct H4 as [vr [rls [rrs]]].
+        destruct H4, H5.
+        injection H6; intros; subst.
+        unfold SetOf_tree_state.
+        rewrite <- H.
+        rewrite H0, H5.
+        simpl; unfold_RELS_tac; tauto.
+      * unfold swap_down_left in H4.
+        destruct H4 as [vl [lls [lrs]]].
+        destruct H4, H5.
+        injection H6; intros; subst.
+        unfold SetOf_tree_state.
+        rewrite <- H.
+        rewrite H0, H5.
+        simpl; unfold_RELS_tac; tauto.
+Qed.
+
+Lemma heap_tree_down_Set_eq: forall (t t': tree_state),
+  heap_tree_down t t' -> SetOf_tree_state t == SetOf_tree_state t'.
+Proof.
+  intros.
+  unfold heap_tree_down in H.
+  revert H; unfold_RELS_tac; intros.
+  destruct H as [t0].
+  destruct H.
+  unfold tree_down_fail in H0.
+  revert H0; unfold_RELS_tac; intros.
+  destruct H0; subst.
+  induction_1n H; [reflexivity|].
+  pose proof tree_down_succeed_Set_eq _ _ H1.
+  revert H2; unfold_RELS_tac; intros.
+  rewrite H2.
+  rewrite IHrt; tauto.
+Qed.
+
+Lemma Pop_from_Set: forall (t t': tree) (s: SetZ),
+  tree_set_rel t s -> (exists d, complete_tree_pop d t) -> MaxHeap t -> tree_pop t t' ->
+  exists s', tree_set_rel t' s' /\
+  ((tree_size t <= 1 /\ s' = ∅) \/ (tree_size t >= 2 /\ (exists x, s' ∪ Singleton x == s /\ MaxSetElement x s))).
+Proof.
+  intros.
+  unfold tree_pop in H2.
+  destruct H2. 1: {
+    destruct H2.
+    exists ∅.
+    split.
+    + rewrite H3.
+      unfold tree_set_rel; simpl.
+      reflexivity.
+    + left. tauto. 
+  }
+  destruct H2.
+  rename H2 into HH.
+  rename H3 into H2.
+  destruct H2 as [v [ls [rs [ts [d0] ] ] ] ].
+  destruct H2, H3, H4; subst.
+  pose proof complete_tree_equality (Node v ls rs).
+  apply H2 in H0.
+  pose proof tree_max_set _ _ H H1 H0.
+  destruct H5; [discriminate|].
+  destruct H5 as [v0 [ls0 [rs0]]].
+  destruct H5.
+  injection H5; intros; subst.
+  pose proof heap_tree_down_Set_eq _ _ H4.
+  unfold SetOf_tree_state in H7; simpl in H7.
+  rewrite Sets_empty_union in H7.
+  exists (SetOf_tree (tree_cut_last ls0 rs0 d0)).
+  split.
+  + unfold tree_set_rel.
+    pose proof tree_compose_set_union (fst ts) (snd ts).
+    revert H8 H7; unfold_RELS_tac; intros.
+    rewrite (H8 x).
+    rewrite H7.
+    tauto.
+  + right.
+    split; [lia|].
+    exists v0.
+    split; [|tauto].
+    pose proof tree_cut_last_set _ _ _ _ HH H3.
+    rewrite H8.
+    unfold tree_set_rel in H.
+    unfold_RELS_tac.
+    tauto.
+Qed.
